simple sketch of rtac.

examples/RTac/Demo.v
@@ -2,7 +2,7 @@ Require Import ExtLib.Core.RelDec.
 Require Import MirrorCore.Lambda.ExprCore.
 Require Import MirrorCore.Lambda.Red.
 Require Import McExamples.Simple.Simple.
-Require Import MirrorCore.RTac.CoreSimple.
+Require Import MirrorCore.RTac.RTac.
 
 Definition open (e : expr typ func)
 : option (   ((typ * (expr typ func -> expr typ func))
@@ -13,67 +13,6 @@ Definition open (e : expr typ func)
     | App (App (Inj Impl) P) Q =>
       Some (inr (P, Q))
     | _ => None
-  end.
-
-Inductive Ctx :=
-| CTop
-| CAll : typ -> Ctx -> Ctx
-| CEx  : typ -> Ctx -> Ctx
-| CHyp : expr typ func -> Ctx -> Ctx.
-
-Fixpoint openGoal' {subst} (g : Goal typ (expr typ func) subst) (ctx : Ctx)
-: Ctx * subst * option (expr typ func) :=
-  match g with
-    | GGoal s e => (ctx,s,e)
-    | GAlls t g => openGoal' g (CAll t ctx)
-    | GExs  t g => openGoal' g (CEx  t ctx)
-    | GHyps h g => openGoal' g (CHyp h ctx)
-  end.
-
-Definition openGoal {subst} g := @openGoal' subst g CTop.
-
-Fixpoint closeGoal {subst} (ctx : Ctx) (g : Goal typ (expr typ func) subst)
-: Goal typ (expr typ func) subst :=
-  match ctx with
-    | CTop => g
-    | CAll t c => closeGoal c (GAlls t g)
-    | CEx t c => closeGoal c (GExs t g)
-    | CHyp t c => closeGoal c (GHyps t g)
-  end.
-
-Section assumption.
-  Context {subst : Type}.
-  Variable (check : expr typ func -> expr typ func -> subst -> option subst).
-
-  Fixpoint findHyp s (ctx : Ctx) (g : expr typ func) {struct ctx}
-  : option subst :=
-    match ctx with
-      | CTop => None
-      | CAll t ctx' => findHyp s ctx' g
-      | CEx  t ctx' => findHyp s ctx' g
-      | CHyp h ctx' => match check g h s with
-                         | None => findHyp s ctx' g
-                         | Some e => Some e
-                       end
-    end.
-
-  Definition ASSUMPTION : rtac typ (expr typ func) subst :=
-    fun g =>
-      let '(ctx,s,gl) := openGoal g in
-      match gl with
-        | None => Some g
-        | Some gl => match findHyp s ctx gl with
-                       | None => None
-                       | Some s => Some (@closeGoal _ ctx (GGoal _ s None))
-                     end
-      end.
-End assumption.
-
-Fixpoint REPEAT {subst} n (tac : rtac typ (expr typ func) subst)
-: rtac typ (expr typ func) subst :=
-  match n with
-    | 0 => TRY tac
-    | S n => TRY (THEN tac (fun x => REPEAT n tac x))
   end.
 
 Let INTRO {subst} :=
