theories/RTac/Intro.v
@@ -1,0 +1,240 @@
+Require Import ExtLib.Structures.Monad.
+Require Import ExtLib.Tactics.
+Require Import MirrorCore.EnvI.
+Require Import MirrorCore.ExprI.
+Require Import MirrorCore.TypesI.
+Require Import MirrorCore.SubstI.
+Require Import MirrorCore.ExprDAs.
+Require Import MirrorCore.RTac.Core.
+
+Require Import MirrorCore.Util.Forwardy.
+
+Set Implicit Arguments.
+Set Strict Implicit.
+
+Section parameterized.
+  Variable typ : Type.
+  Variable expr : Type.
+  Variable subst : Type.
+
+  Variable RType_typ : RType typ.
+  Variable Expr_expr : Expr RType_typ expr.
+  Variable Typ0_Prop : Typ0 _ Prop.
+  Variable Subst_subst : Subst subst expr.
+  Variable SubstOk_subst : @SubstOk _ _ _ _ Expr_expr Subst_subst.
+
+  Section at_bottom.
+    Variable m : Type -> Type.
+    Context {Monad_m : Monad m}.
+    Variable gt : list typ -> list typ -> subst -> option expr -> m (Goal typ expr subst).
+
+    Let under (gt : Goal typ expr subst -> Goal typ expr subst)
+        (x : m (Goal typ expr subst)) : m (Goal typ expr subst) :=
+      bind x (fun x => ret (gt x)).
+
+    Fixpoint at_bottom tus tvs (g : Goal typ expr subst)
+    : m (Goal typ expr subst) :=
+      match g with
+        | GAlls x g' => under (GAlls x) (at_bottom tus (tvs ++ x :: nil) g')
+        | GExs  x g' => under (GExs  x) (at_bottom (tus ++ x :: nil) tvs g')
+        | GHyps x g' => under (GHyps x) (at_bottom tus tvs g')
+        | GGoal s e => gt tus tvs s e
+      end.
+  End at_bottom.
+
+  Variable substV : (nat -> option expr) -> expr -> expr.
+  Variable Var : nat -> expr.
+
+  Definition INTRO
+             (open : expr -> option ((typ * (expr -> expr)) + (expr * expr)))
+  : rtac typ expr subst :=
+    fun g => at_bottom (m := option)
+                       (fun tus tvs s g =>
+                          match g with
+                            | None => None
+                            | Some g =>
+                              match open g with
+                                | None => None
+                                | Some (inl (t, g')) =>
+                                  let nv := length tvs in
+                                  Some (GAlls t (GGoal s (Some (g' (Var nv)))))
+                                | Some (inr (t, g')) =>
+                                  Some (GHyps t (GGoal s (Some g')))
+                              end
+                          end)
+               nil nil g.
+
+  Definition open_sound (open : expr -> option ((typ + expr) * expr)) : Prop :=
+    forall tus tvs e eD h e',
+      open e = Some (h,e') ->
+      propD tus tvs e = Some eD ->
+      match h with
+        | inl t =>
+          exists eD',
+          propD tus (t :: tvs) e' = Some eD' /\
+          forall us vs,
+            (eD us vs) -> (forall x : typD nil t, eD' us (HList.Hcons x vs))
+        | inr h =>
+          False
+      end.
+
+(*
+  Lemma _impls_sem
+  : forall ls P,
+      _impls ls P <-> (Forall (fun x => x) ls -> P).
+  Proof.
+    induction ls; simpl; intros.
+    + intuition.
+    + rewrite IHls. intuition.
+      inversion H0. eapply H; eauto.
+  Qed.
+  Lemma _exists_iff
+  : forall ls P Q,
+      (forall x, P x <-> Q x) ->
+      (@_exists ls P <-> @_exists ls Q).
+  Proof.
+    clear.
+    induction ls; simpl; intros.
+    + eapply H.
+    + apply exists_iff; intro. eapply IHls.
+      intro; eapply H.
+  Qed.
+  Lemma _forall_iff
+  : forall ls P Q,
+      (forall x, P x <-> Q x) ->
+      (@_foralls ls P <-> @_foralls ls Q).
+  Proof.
+    clear.
+    induction ls; simpl; intros.
+    + eapply H.
+    + apply forall_iff; intro. eapply IHls.
+      intro; eapply H.
+  Qed.
+
+  Lemma at_bottom_sound_option
+  : forall goal tus tvs f goal',
+      (forall tus' tvs' s e e',
+         f (tus ++ tus') (tvs ++ tvs') s e = Some e' ->
+         WellFormed_subst s ->
+         match goalD (tus ++ tus') (tvs ++ tvs') (GGoal s e)
+             , goalD (tus ++ tus') (tvs ++ tvs') e'
+         with
+           | None , _ => True
+           | Some _ , None => False
+           | Some g , Some g' =>
+             forall us vs,
+               g' us vs -> g us vs
+         end) ->
+      at_bottom f tus tvs goal = Some goal' ->
+      forall (Hwf : WellFormed_goal goal),
+      match goalD tus tvs goal
+          , goalD tus tvs goal'
+      with
+        | None , _ => True
+        | Some _ , None => False
+        | Some g , Some g' =>
+          forall us vs,
+            g' us vs -> g us vs
+      end.
+  Proof.
+    induction goal; simpl; intros.
+    { forwardy. inv_all; subst.
+      eapply IHgoal in H0; clear IHgoal; auto.
+      { simpl. forward. auto. }
+      { intros.
+        specialize (H tus' (t :: tvs') s e).
+        rewrite app_ass in H1. simpl in *.
+        eapply H in H1; clear H; auto.
+        forward.
+        rewrite substD_conv
+           with (pfu := eq_refl _) (pfv := eq_sym (HList.app_ass_trans _ _ _)) in H.
+        unfold propD in *.
+        rewrite exprD'_typ0_conv with (pfu := eq_refl _)
+             (pfv := eq_sym (HList.app_ass_trans _ _ _)) in H.
+        simpl in *.
+        unfold ResType in *.
+        autorewrite with eq_rw in *.
+        destruct e; forwardy.
+        { inv_all; subst.
+          rewrite H in *.
+          autorewrite with eq_rw in H3.
+          forwardy.
+          rewrite H3 in *.
+          inv_all; subst.
+          rewrite goalD_conv with (pfu := eq_refl)
+                                  (pfv := eq_sym (HList.app_ass_trans _ _ _)).
+          simpl.
+          forwardy.
+          autorewrite with eq_rw.
+          rewrite H1.
+          intros us vs. autorewrite with eq_rw.
+          clear - H4.
+          match goal with
+            | |- _ _ match ?X with _ => _ end ->
+                 _ _ match ?Y with _ => _ end /\
+                 _ _ match ?Z with _ => _ end =>
+              change X with Y ; change Z with Y ; destruct Y
+          end.
+          eauto. }
+        { rewrite H in *.
+          rewrite goalD_conv with (pfu := eq_refl)
+                                  (pfv := eq_sym (HList.app_ass_trans _ _ _)).
+          simpl.
+          forwardy.
+          autorewrite with eq_rw.
+          rewrite H1. intros.
+          inv_all; subst.
+          revert H6.
+          match goal with
+            | |- match ?X with _ => _ end _ _ ->
+                 match ?Y with _ => _ end _ _ =>
+              change Y with X ; destruct X
+          end. auto. } } }
+    { forwardy; inv_all; subst.
+      eapply IHgoal in H0; clear IHgoal; auto.
+      + simpl; forward; eauto.
+        destruct H3. eauto.
+      + intros.
+        rewrite goalD_conv
+           with (pfu := eq_sym (HList.app_ass_trans _ _ _))
+                (pfv := eq_refl).
+        autorewrite with eq_rw.
+        simpl. forward.
+        rewrite HList.app_ass_trans in H1.
+        simpl in H1.
+        eapply H in H1; clear H; eauto.
+        destruct e; forward.
+        - inv_all; subst.
+          revert H7. autorewrite with eq_rw.
+          eauto.
+        - inv_all; subst.
+          revert H6. autorewrite with eq_rw.
+          eauto. }
+    { forwardy; inv_all; subst.
+      eapply IHgoal in H0; clear IHgoal; eauto.
+      + simpl; forward; eauto.
+        inv_all. subst.
+        eapply _impls_sem; intro.
+        eapply _impls_sem in H5; eauto. }
+    { specialize (H nil nil s o goal').
+      simpl in H.
+      repeat rewrite HList.app_nil_r_trans in H.
+      eapply H in H0; clear H; auto. }
+  Qed.
+
+(*
+  Theorem INTRO_sound
+  : forall open, open_sound open ->
+                 rtac_sound nil nil (INTRO open).
+  Proof.
+    unfold rtac_sound, INTRO.
+    intros.
+    eapply at_bottom_sound_option in H0; eauto.
+(*
+    { destruct (goalD nil nil g); destruct (goalD nil nil g'); auto.
+*)
+  Abort.
+*)
+*)
+
+End parameterized.
